src/ADTRefinement/BuildADTRefinements/RefineAllMethods.v
@@ -19,65 +19,45 @@ Section RefineAllMethods.
 
   Variable Rep : Type. (* The old representation type. *)
 
-  Lemma refineConstructor_eq_sound :
-    forall cSig
-           (cDef refinedCDef : constructorType Rep cSig),
-      refineConstructor_eq Rep cDef refinedCDef ->
-      let H := refinedCDef in refineConstructor eq cDef H.
-  Proof.
-    induction cSig; simpl; intros.
-    - etransitivity.
-      + apply refine_under_bind; intros.
-        refine pick val a; eauto; finish honing.
-      + simpl; autorewrite with monad laws; eauto.
-    - eapply IHcSig; eauto.
-  Qed.
-
   Lemma refineMethod_eq_sound :
-    forall Dom Cod
-           (cDef refinedCDef : methodType Rep Dom Cod),
-      refineMethod_eq cDef refinedCDef ->
-      let H := refinedCDef in refineMethod eq cDef H.
+    forall arity Dom Cod
+           (cDef refinedCDef : methodType arity Rep Dom Cod),
+      refineMethod_eq _ arity cDef refinedCDef ->
+      let H := refinedCDef in refineMethod eq _ cDef H.
   Proof.
-    unfold refineMethod; simpl; intros; subst.
-    induction Dom; simpl; intros.
-    - destruct Cod; simpl in *.
-      + etransitivity.        
-        * apply refine_under_bind; intros.
+    simpl; intros; subst.
+    induction arity; simpl; intros.
+    - induction Dom; simpl; intros.
+      + destruct Cod; simpl in *.
+        * etransitivity.        
+          apply refine_under_bind; intros.
           refine pick val (fst a); eauto; simplify with monad laws.
           destruct a; simpl; finish honing.
-        * simpl; autorewrite with monad laws; eapply H.
-      + etransitivity.
-        * apply refine_under_bind; intros.
+          simpl; autorewrite with monad laws; eapply H.
+        * etransitivity.
+          apply refine_under_bind; intros.
           refine pick val a; eauto; simpl; finish honing.
-        * simpl; autorewrite with monad laws; eapply H.
-    - eapply (IHDom (fun r_n => cDef r_n d) (fun r_n => refinedCDef r_n d)).
-      unfold refineMethod_eq; intros; eapply H.
+          simpl; autorewrite with monad laws; eapply H.
+      + eapply (IHDom (cDef d) (refinedCDef d)).
+        unfold refineMethod_eq; intros; eapply H.
+    - subst; simpl in *; eauto.
   Qed.
 
   Lemma refineADT_BuildADT_Rep_refine_All_eq
-        {n n'}
-        (consSigs : Vector.t consSig n)
-        (methSigs : Vector.t methSig n')
-        (consDefs : ilist (B := @consDef Rep) consSigs)
+        {n}
+        (methSigs : Vector.t methSig n)
         (methDefs : ilist (B := @methDef Rep) methSigs)
-        (refined_consDefs : ilist (B := @consDef Rep) consSigs)
         (refined_methDefs : ilist (B := @methDef Rep) methSigs)
-    : Iterate_Ensemble_BoundedIndex (fun idx => refineConstructor_eq _ (ith consDefs idx) (ith refined_consDefs idx))
-      -> Iterate_Ensemble_BoundedIndex (fun idx => refineMethod_eq (ith methDefs idx) (ith refined_methDefs idx))
+    : Iterate_Ensemble_BoundedIndex (fun idx => refineMethod_eq _ _ (ith methDefs idx) (ith refined_methDefs idx))
       -> refineADT
-           (BuildADT consDefs methDefs)
-           (BuildADT refined_consDefs refined_methDefs).
+           (BuildADT methDefs)
+           (BuildADT refined_methDefs).
   Proof.
     intros; eapply refineADT_BuildADT_Rep_refine_All with (AbsR := eq).
-    - revert H; clear; induction consSigs; simpl in *;
-      destruct consDefs; destruct refined_consDefs; try econstructor; simpl.
-      intros; destruct H; destruct prim_fst; destruct prim_fst0; econstructor; eauto.
-      destruct h; eapply (@refineConstructor_eq_sound consDom); eauto.
-    - revert H0; clear; induction methSigs; simpl in *;
+    - revert H; clear; induction methSigs; simpl in *;
       destruct methDefs; destruct refined_methDefs; try econstructor; simpl.
-      intros; destruct H0; destruct prim_fst; destruct prim_fst0; econstructor; eauto.
-      destruct h; eapply (@refineMethod_eq_sound methDom methCod); eauto.
+      intros; destruct H; destruct prim_fst; destruct prim_fst0; econstructor; eauto.
+      destruct h; eapply (@refineMethod_eq_sound _ methDom methCod); eauto.
   Qed.
 
 End RefineAllMethods.
@@ -100,17 +80,11 @@ Ltac refineEachMethod :=
         (@methDef Rep)
         methSigs
         ltac:(fun rMeths =>
-                ilist_of_evar1
-                  (@consDef Rep)
-                  consSigs
-                  ltac:(fun rCons =>
-                          eapply refineADT_BuildADT_Rep_refine_All_eq
-                          with (refined_methDefs := rMeths)
-                                 (refined_consDefs := rCons)
-             )); unfold refineMethod_eq;
+                eapply refineADT_BuildADT_Rep_refine_All_eq
+                with (refined_methDefs := rMeths)                       
+             ); unfold refineMethod_eq;
     simpl; repeat apply Build_prim_and; intros; 
-    first [instantiate (1 := {| consBody :=  _ |})
-          | instantiate (1 := {| methBody :=  _ |})
+    first [ instantiate (1 := {| methBody :=  _ |})
           | eauto ]; simpl
   end.
 
